hadl-formal.md
@@ -1,0 +1,19 @@
+This is the Schema self-healing rule. The crucial step is that an error in typechecking the continuation p is what drives self-healing.
+
+Differences:
+\Gamma |- v: \tau => ok | err(e)
+raise(e)
+Sigma: Now stores only errors and becomes empty on success
+
+
+SUCCESS
+v \in O(s, \Sigma, \tau)
+\Gamma |- v: \tau => ok
+\Gamma, x: Schema |- p: \tau' => ok
+<\Gamma, \Sigma, \Pi, let x: Schema = gen s; p> -> <\Gamma, [], \Pi, p[v/x]>
+
+SELF-HEAL
+v \in O(s, \Sigma, Schema)
+\Gamma |- v: Schema => ok
+\Gamma, x: Schema |- p: \tau' => err(e)
+<\Gamma, \Sigma, \Pi, let x: Schema = gen s; p> -> <\Gamma, \Sigma \cdot e, \Pi, let x: Schema = gen s; p>
